Distinction_Implies_Winning_Budgets.thy
@@ -350,7 +350,7 @@ proof-
           using case_assms(1) subset_form by auto
         have eu'_comp: \<open>eu' = (expr_pr_inner (Conj I \<psi>s)) - (E 0 0 1 0 0 0 0 0)\<close>
           unfolding eu'_def
-          by (auto simp add: bot_enat_def) (metis (no_types, lifting) SUP_cong energy.sel image_image)+
+          by (auto simp add: bot_enat_def image_image)
         with expr_lower have eu'_characterization: \<open>Some eu' = (subtract_fn 0 0 1 0 0 0 0 0) (expr_pr_inner (Conj I \<psi>s))\<close>
           by presburger
         have \<open>\<forall>g'. spectroscopy_moves (Defender_Conj p Q) g' \<noteq> None
